scratch/ConThunkFieldUnsound.v
@@ -29,6 +29,7 @@ Definition SoundnessStatement : Prop :=
     contains_env σ S Γs Γc ->
     contains σ S e_sym e_con ->
     concore_expr e_con ->
+    closed_program Γc e_con ->
     Φ ; Γs ⊢ e_sym ⇓ v_sym ->
     exists v_con, Γc ⊢ᶜ e_con ⇓ᶜ v_con /\ contains σ S v_sym v_con.
 
@@ -57,6 +58,9 @@ Qed.
 
 Lemma thunk_field_program_concore : concore_expr thunk_field_program.
 Proof. repeat constructor. Qed.
+
+Lemma thunk_field_program_closed : closed_program · thunk_field_program.
+Proof. split; [constructor | repeat constructor]. Qed.
 
 Lemma branch_field_symbolic_value : forall Φ c,
   Φ ; · ⊢ branch_field_program c ⇓ branch_field_value c.
@@ -93,7 +97,7 @@ Proof.
   pose proof (branch_field_contains_thunk_field σ S c Hy Hc) as Hcont.
   destruct Hc as [pc [_ Hm]].
   destruct (Hsound pc · · σ S _ thunk_field_program _ Hm (Cont_Env_Empty _ _) Hcont
-              thunk_field_program_concore (branch_field_symbolic_value pc c))
+              thunk_field_program_concore thunk_field_program_closed (branch_field_symbolic_value pc c))
     as [v [Hv Hcv]].
   rewrite (thunk_field_concrete_value v Hv) in Hcv.
   exact (old_symbolic_value_misses_concrete_value σ S c Hold Hcv).
