scratch/ReducePrimOverheadNeedsSlack.v
@@ -1,4 +1,4 @@
-From SymCoreTheory Require Import SymCore ConCore BranchLaws CostLaws Model.
+From SymCoreTheory Require Import SymCore ConCore CostLaws Model.
 From Stdlib Require Import Strings.String Lists.List Bool.Bool Arith.PeanoNat Lia.
 Import ListNotations.
 Open Scope string_scope.
@@ -22,6 +22,12 @@ Proof.
   - exact (ContK_App sigma_all all_symvars 0 0 _ _ _ _ (ContK_PrimOp _ _ PAnd) IH).
 Qed.
 
+Lemma and_tower_closed : forall n, closed_term (and_tower n lit_true).
+Proof.
+  induction n as [| n IH]; simpl; [apply Scoped_Lit |].
+  apply Scoped_App; [apply Scoped_PrimOp | exact IH].
+Qed.
+
 Lemma and_tower_facts : forall n e,
   flat e = true ->
   flat (and_tower n e) = true /\ smt_size (and_tower n e) = 2 * n + smt_size e /\
@@ -41,9 +47,10 @@ Proof.
   change (model_reduce_prim PNot (a :: nil) = fold_leaf (EApp (EPrimOp PNot) a)).
   unfold model_reduce_prim.
   rewrite split_args_not_if by (constructor; [apply flat_not_if; exact Hf | constructor]).
-  unfold reduce_unbranched, op_spine. cbn [length model_arity Nat.eqb fold_left].
-  rewrite lift_flat by (simpl; rewrite Hf; reflexivity).
-  reflexivity.
+  unfold simplify_unbranched, simplify.
+  destruct (forallb smt_term (a :: nil) && negb (forallb smt_ground (a :: nil)));
+    cbn iota; unfold reduce_unbranched, op_spine; cbn [length model_arity Nat.eqb fold_left];
+    rewrite lift_flat by (simpl; rewrite Hf; reflexivity); reflexivity.
 Qed.
 
 Lemma app_contains_k_lit : forall σ S k f a l,
@@ -52,6 +59,7 @@ Proof. intros σ S k f a l H. inversion H; subst. reflexivity. Qed.
 
 Theorem model_breaks_constant_slack : forall c,
   ~ (forall σ S p ks args_s args_c,
+       Forall closed_term args_c ->
        Forall3 (contains_k σ S) ks args_s args_c ->
        exists k', k' <= list_sum ks + c /\
          contains_k σ S k' (reduce_prim p args_s) (reduce_prim p args_c)).
@@ -59,6 +67,7 @@ Proof.
   intros c Hlaw.
   destruct (Hlaw sigma_all all_symvars PNot (0 :: nil)
               (and_tower c sym_x :: nil) (and_tower c lit_true :: nil)
+              (Forall_cons _ (and_tower_closed c) (Forall_nil _))
               (Forall3_cons _ _ _ _ _ _ _ (and_tower_contains_k c) (Forall3_nil _)))
     as [k' [Hle Hc]].
   destruct (and_tower_facts c sym_x eq_refl) as [Hfs [Hss [Hgs _]]].
@@ -94,8 +103,11 @@ Proof.
   rewrite Hf, Hs, Hg. split; [reflexivity | split; [lia | reflexivity]].
 Qed.
 
-Lemma lit_true_models : models_cond sigma_all all_symvars lit_true.
-Proof. exists (@PCLit model_sorts true). split; [intros Γ _; reflexivity | reflexivity]. Qed.
+Lemma sym_x_models : models_cond sigma_all all_symvars sym_x.
+Proof.
+  exists (@PCVar model_sorts "x"). split; [| reflexivity].
+  intros Γ Hfree. simpl. rewrite (Hfree "x" eq_refl). reflexivity.
+Qed.
 
 Theorem model_ite_needs_arm_sizes : forall c,
   ~ (forall σ S k ec et ef pt pf l,
@@ -107,19 +119,23 @@ Proof.
   intros c Hlaw.
   destruct (not_tower_denotes c) as [pf Hpf].
   destruct (not_tower_facts c) as [Hf [Hs Hg]].
-  assert (Hc : contains_k sigma_all all_symvars 2 (EIf lit_true lit_true (not_tower c)) lit_true)
-    by exact (ContK_If_True sigma_all all_symvars 0 lit_true lit_true (not_tower c) lit_true
-                lit_true_models (ContK_Lit _ _ true)).
-  destruct (Hlaw sigma_all all_symvars 2 lit_true lit_true (not_tower c) (@PCLit model_sorts true) pf true
+  assert (Hc : contains_k sigma_all all_symvars 2 (EIf sym_x lit_true (not_tower c)) lit_true)
+    by exact (ContK_If_True sigma_all all_symvars 0 sym_x lit_true (not_tower c) lit_true
+                sym_x_models (ContK_Lit _ _ true)).
+  destruct (Hlaw sigma_all all_symvars 2 sym_x lit_true (not_tower c) (@PCLit model_sorts true) pf true
               (fun Γ _ => eq_refl) Hpf Hc) as [k' [Hle Hk']].
   change (contains_k sigma_all all_symvars k'
-            (model_reduce_prim PIte (lit_true :: lit_true :: not_tower c :: nil)) (ELit true)) in Hk'.
+            (model_reduce_prim PIte (sym_x :: lit_true :: not_tower c :: nil)) (ELit true)) in Hk'.
   unfold model_reduce_prim in Hk'.
   rewrite split_args_not_if in Hk'
     by (repeat constructor; apply flat_not_if; exact Hf).
+  assert (Hs0 : simplify PIte (sym_x :: lit_true :: not_tower c :: nil) = None).
+  { unfold simplify. destruct (_ && _); [| reflexivity].
+    destruct c; reflexivity. }
+  unfold simplify_unbranched in Hk'. rewrite Hs0 in Hk'.
   unfold reduce_unbranched, op_spine in Hk'. cbn [length model_arity Nat.eqb fold_left] in Hk'.
   rewrite lift_flat in Hk' by (simpl; rewrite Hf; reflexivity).
-  rewrite fold_leaves_not_if in Hk' by reflexivity. unfold fold_leaf in Hk'. cbn [smt_ground is_op_app andb] in Hk'. rewrite Hg in Hk'.
+  rewrite fold_leaves_not_if in Hk' by reflexivity. unfold fold_leaf in Hk'. cbn [smt_ground is_op_app andb] in Hk'.
   simpl in Hk'.
   apply app_contains_k_lit in Hk'. simpl in Hk'. rewrite Hs in Hk'. lia.
 Qed.
